SmtExpr.v
@@ -65,6 +65,6 @@ with eval_smt_arith (e : SmtArithExpr) (v : SmtValuation) : uint8 :=
 
 (* Apply SmtValuation f to every entry in the symbolic state across all 3 maps *)
 Definition eval_sym_state (s: ProgramState SmtArithExpr) (f : SmtValuation) : ProgramState uint8 :=
-  {| header_map := fun h => eval_smt_arith (header_map s h) f;
-     ctrl_plane_map := fun c => eval_smt_arith (ctrl_plane_map s c) f;
-     state_var_map := fun sv => eval_smt_arith (state_var_map s sv) f |}.
+  {| header_map := fun h => eval_smt_arith (lookup_hdr s h) f;
+     ctrl_plane_map := fun c => eval_smt_arith (lookup_ctrl s c) f;
+     state_var_map := fun sv => eval_smt_arith (lookup_state s sv) f |}.
